Core/Vec.lean
@@ -11,6 +11,9 @@ theorem Vec.length_list : {v : Vec α n} -> v.list.length = n
 | #() => by simp [list]
 | .cons x xs => by simp [list, length_list (v := xs)]
 
+@[grind =]
+theorem Vec.get_to {v : Fun.Vec α n} : v.to[i] = v i := sorry
+
 def Vec.rmap [RenMap S T] (r : Ren T) : Vec S n -> Vec S n
 | .nil => .nil
 | .cons x tl => x⟨r⟩ :: rmap r tl
